James C - yet more cleanup

isabelle/Chapter08_1_Language.thy
@@ -1,5 +1,5 @@
 theory Chapter08_1_Language
-imports DeBruijnEnvironment
+imports Name
 begin
 
 datatype type = 
@@ -8,39 +8,29 @@ datatype type =
 | Arrow type type
 
 datatype expr = 
-  Var var
+  Var name
 | Num int
 | Str string
 | Plus expr expr
 | Times expr expr
 | Cat expr expr
 | Len expr
-| Let expr expr
-| Lam type expr
+| Let expr "name \<Rightarrow> expr option"
+| Lam type "name \<Rightarrow> expr option"
 | Appl expr expr
 
-primrec insert :: "var \<Rightarrow> expr \<Rightarrow> expr" where 
-  "insert n (Var v) = Var (incr n v)"
-| "insert n (Num x) = Num x"
-| "insert n (Str s) = Str s"
-| "insert n (Plus e1 e2) = Plus (insert n e1) (insert n e2)"
-| "insert n (Times e1 e2) = Times (insert n e1) (insert n e2)"
-| "insert n (Cat e1 e2) = Cat (insert n e1) (insert n e2)"
-| "insert n (Len e) = Len (insert n e)"
-| "insert n (Let e1 e2) = Let (insert n e1) (insert (next n) e2)"
-| "insert n (Lam t e) = Lam t (insert (next n) e)"
-| "insert n (Appl e1 e2) = Appl (insert n e1) (insert n e2)"
-
-primrec subst :: "expr \<Rightarrow> var \<Rightarrow> expr \<Rightarrow> expr" where 
-  "subst e' n (Var x) = (if x = n then e' else Var (subr n x))"
+primrec subst :: "expr \<Rightarrow> name \<Rightarrow> expr \<Rightarrow> expr" where 
+  "subst e' n (Var x) = (if x = n then e' else Var x)"
 | "subst e' n (Num x) = Num x"
 | "subst e' n (Str s) = Str s"
 | "subst e' n (Plus e1 e2) = Plus (subst e' n e1) (subst e' n e2)"
 | "subst e' n (Times e1 e2) = Times (subst e' n e1) (subst e' n e2)"
 | "subst e' n (Cat e1 e2) = Cat (subst e' n e1) (subst e' n e2)"
 | "subst e' n (Len e) = Len (subst e' n e)"
-| "subst e' n (Let e1 e2) = Let (subst e' n e1) (subst (insert first e') (next n) e2)"
-| "subst e' n (Lam t e) = Lam t (subst (insert first e') (next n) e)"
+| "subst e' n (Let e1 e2) =
+    Let (subst e' n e1) (\<lambda>x. if x = n then None else map_option (subst e' n) (e2 x))"
+| "subst e' n (Lam t e) = 
+    Lam t (\<lambda>x. if x = n then None else map_option (subst e' n) (e x))"
 | "subst e' n (Appl e1 e2) = Appl (subst e' n e1) (subst e' n e2)"
 
 end
