isabelle/Chapter08_2_Typechecking.thy
@@ -3,7 +3,7 @@ imports Chapter08_1_Language
 begin
 
 inductive typecheck :: "type env \<Rightarrow> expr \<Rightarrow> type \<Rightarrow> bool" where 
-  tc_var [simp]: "lookup gam x = Some t \<Longrightarrow> typecheck gam (Var x) t"
+  tc_var [simp]: "gam x = Some t \<Longrightarrow> typecheck gam (Var x) t"
 | tc_str [simp]: "typecheck gam (Str s) StrType"
 | tc_num [simp]: "typecheck gam (Num n) NumType"
 | tc_plus [simp]: "typecheck gam e1 NumType \<Longrightarrow> typecheck gam e2 NumType \<Longrightarrow>
@@ -13,9 +13,11 @@ inductive typecheck :: "type env \<Rightarrow> expr \<Rightarrow> type \<Rightar
 | tc_cat [simp]: "typecheck gam e1 StrType \<Longrightarrow> typecheck gam e2 StrType \<Longrightarrow>
     typecheck gam (Cat e1 e2) StrType"
 | tc_len [simp]: "typecheck gam e StrType \<Longrightarrow> typecheck gam (Len e) NumType"
-| tc_let [simp]: "typecheck gam e1 t1 \<Longrightarrow> typecheck (extend gam t1) e2 t2 \<Longrightarrow>
-    typecheck gam (Let e1 e2) t2"
-| tc_lam [simp]: "typecheck (extend gam t1) e t2 \<Longrightarrow> typecheck gam (Lam t1 e) (Arrow t1 t2)"
+| tc_let [simp]: "typecheck gam e1 t1 \<Longrightarrow> 
+    (\<And>n e2'. n \<notin> dom gam \<Longrightarrow> e2 n = Some e2' \<Longrightarrow> typecheck (gam (n \<mapsto> t1)) e2' t2) \<Longrightarrow> 
+      typecheck gam (Let e1 e2) t2"
+| tc_lam [simp]: "(\<And>n e'. n \<notin> dom gam \<Longrightarrow> e n = Some e' \<Longrightarrow> typecheck (gam (n \<mapsto> t1)) e' t2) \<Longrightarrow> 
+    typecheck gam (Lam t1 e) (Arrow t1 t2)"
 | tc_appl [simp]: "typecheck gam e1 (Arrow t2 t) \<Longrightarrow> typecheck gam e2 t2 \<Longrightarrow>
     typecheck gam (Appl e1 e2) t"
 
@@ -30,11 +32,81 @@ inductive_cases [elim!]: "typecheck gam (Let e1 e2) t"
 inductive_cases [elim!]: "typecheck gam (Lam t1 e) t"
 inductive_cases [elim!]: "typecheck gam (Appl e1 e2) t"
 
-lemma [simp]: "typecheck gam e t \<Longrightarrow> n in gam \<Longrightarrow> typecheck (extend_at n gam t') (insert n e) t"
-  by (induction gam e t arbitrary: n rule: typecheck.induct) fastforce+
+lemma [elim]: "typecheck gam e t \<Longrightarrow> n \<notin> dom gam \<Longrightarrow> typecheck (gam(n \<mapsto> t')) e t"
+  proof (induction gam e t rule: typecheck.induct)
+  case (tc_var gam x t)
+    hence "(gam(n \<mapsto> t')) x = Some t" by auto
+    thus ?case by auto
+  next case tc_str
+    thus ?case by simp
+  next case tc_num
+    thus ?case by simp
+  next case tc_plus
+    thus ?case by simp
+  next case tc_times
+    thus ?case by simp
+  next case tc_cat
+    thus ?case by simp
+  next case tc_len
+    thus ?case by simp
+  next case (tc_let gam e1 t1 e2 t2)
+    hence "typecheck (gam(n \<mapsto> t')) e1 t1" by fastforce
+    moreover have "\<And>m e2'. m \<notin> dom (gam(n \<mapsto> t')) \<Longrightarrow> e2 n = Some e2' \<Longrightarrow> typecheck ((gam(n \<mapsto> t')) (m \<mapsto> t1)) e2' t2"
+      proof -
+        fix m e2'
+        assume "m \<notin> dom (gam(n \<mapsto> t'))"
+           and "e2 n = Some e2'"
+        
 
-lemma [simp]: "typecheck (extend_at n gam t') e t \<Longrightarrow> n in gam \<Longrightarrow> typecheck gam e' t' \<Longrightarrow>
+        show "typecheck (gam(n \<mapsto> t', m \<mapsto> t1)) e2' t2" by simp
+      qed
+    ultimately show ?case try
+  next case tc_lam
+    thus ?case by simp
+  next case tc_appl
+    thus ?case by simp
+  qed 
+
+lemma [simp]: "typecheck (gam(n \<mapsto> t')) e t \<Longrightarrow> typecheck gam e' t' \<Longrightarrow>
     typecheck gam (subst e' n e) t"
-  by (induction "extend_at n gam t'" e t arbitrary: n gam t' e' rule: typecheck.induct) fastforce+
+  proof (induction "gam(n \<mapsto> t')" e t arbitrary: n gam t' e' rule: typecheck.induct)
+  case tc_var
+    thus ?case by auto
+  next case tc_str
+    thus ?case by simp
+  next case tc_num
+    thus ?case by simp
+  next case tc_plus
+    thus ?case by simp
+  next case tc_times
+    thus ?case by simp
+  next case tc_cat
+    thus ?case by simp
+  next case tc_len
+    thus ?case by simp
+  next case (tc_let e1 t1 e2 t2)
+    hence "typecheck gam (subst e' n e1) t1" by simp
+    moreover have "\<And>m. m \<notin> dom gam \<Longrightarrow> typecheck (gam (m \<mapsto> t1)) (subst e' n (e2 m)) t2"
+      proof -
+        fix m
+        assume "m \<notin> dom gam"
+        from tc_let have "typecheck gam e' t'" by simp
+
+
+        have X: "m \<notin> dom (gam(n \<mapsto> t'))" by simp
+
+
+        have Y: "gam(n \<mapsto> t', m \<mapsto> t1) = gam (m \<mapsto> t1, n \<mapsto> t')" by simp
+
+
+        have "typecheck (gam (m \<mapsto> t1)) e' t'" by simp
+        with X Y tc_let show "typecheck (gam (m \<mapsto> t1)) (subst e' n (e2 m)) t2" by simp
+      qed
+    ultimately show ?case by simp
+  next case tc_lam
+    thus ?case by simp
+  next case tc_appl
+    thus ?case by simp
+  qed 
 
 end
