isabelle/Chapter15_2_Language.thy
@@ -1,0 +1,80 @@
+theory Chapter15_2_Language
+imports Chapter15_1_Types
+begin
+
+datatype expr = 
+  Var var
+| Zero
+| Suc expr
+| Iter expr expr expr
+| Lam type expr
+| Appl expr expr
+| Triv
+| Pair expr expr
+| ProjL expr
+| ProjR expr
+| Abort type expr
+| Case expr expr expr
+| InL type type expr
+| InR type type expr
+| Strgen type expr expr expr
+| Hd expr
+| Tl expr
+| Fold type expr
+| Rec type expr expr
+| Unfold type expr
+| Gen type expr expr
+
+primrec insert :: "var \<Rightarrow> expr \<Rightarrow> expr" where 
+  "insert n (Var v) = Var (incr n v)"
+| "insert n Zero = Zero"
+| "insert n (Suc e) = Suc (insert n e)"
+| "insert n (Iter et e0 es) = Iter (insert n et) (insert n e0) (insert (next n) es)"
+| "insert n (Lam t e) = Lam t (insert (next n) e)"
+| "insert n (Appl e1 e2) = Appl (insert n e1) (insert n e2)"
+| "insert n Triv = Triv"
+| "insert n (Pair e1 e2) = Pair (insert n e1) (insert n e2)"
+| "insert n (ProjL e) = ProjL (insert n e)"
+| "insert n (ProjR e) = ProjR (insert n e)"
+| "insert n (Abort t e) = Abort t (insert n e)"
+| "insert n (Case et el er) = Case (insert n et) (insert (next n) el) (insert (next n) er)"
+| "insert n (InL t1 t2 e) = InL t1 t2 (insert n e)"
+| "insert n (InR t1 t2 e) = InR t1 t2 (insert n e)"
+| "insert n (Strgen t e e1 e2) = Strgen t (insert n e) (insert (next n) e1) (insert (next n) e2)"
+| "insert n (Hd e) = Hd (insert n e)"
+| "insert n (Tl e) = Tl (insert n e)"
+| "insert n (Fold t e) = Fold t (insert n e)"
+| "insert n (Rec t e e1) = Rec t (insert n e) (insert (next n) e1)"
+| "insert n (Fold t e) = Fold t (insert n e)"
+| "insert n (Fold t e) = Fold t (insert n e)"
+
+primrec subst :: "expr \<Rightarrow> var \<Rightarrow> expr \<Rightarrow> expr" where 
+  "subst e' n (Var v) = (if v = n then e' else Var (subr n v))"
+| "subst e' n Zero = Zero"
+| "subst e' n (Suc e) = Suc (subst e' n e)"
+| "subst e' n (Iter et e0 es) = 
+    Iter (subst e' n et) (subst e' n e0) (subst (insert first e') (next n) es)"
+| "subst e' n (Lam t e) = Lam t (subst (insert first e') (next n) e)"
+| "subst e' n (Appl e1 e2) = Appl (subst e' n e1) (subst e' n e2)"
+| "subst e' n Triv = Triv"
+| "subst e' n (Pair e1 e2) = Pair (subst e' n e1) (subst e' n e2)"
+| "subst e' n (ProjL e) = ProjL (subst e' n e)"
+| "subst e' n (ProjR e) = ProjR (subst e' n e)"
+| "subst e' n (Abort t e) = Abort t (subst e' n e)"
+| "subst e' n (Case et el er) = 
+    Case (subst e' n et) (subst (insert first e') (next n) el) 
+      (subst (insert first e') (next n) er)"
+| "subst e' n (InL t1 t2 e) = InL t1 t2 (subst e' n e)"
+| "subst e' n (InR t1 t2 e) = InR t1 t2 (subst e' n e)"
+| "subst e' n (Strgen t e e1 e2) = Strgen t (subst e' n e) (subst (insert first e') (next n) e1) 
+      (subst (insert first e') (next n) e2)"
+| "subst e' n (Hd e) = Hd (subst e' n e)"
+| "subst e' n (Tl e) = Tl (subst e' n e)"
+
+lemma [simp]: "canswap m n \<Longrightarrow> insert m (insert n e) = insert (next n) (insert m e)"
+  by (induction e arbitrary: n m) simp_all
+
+lemma [simp]: "subst e' n (insert n e) = e"
+  by (induction e arbitrary: n e') simp_all
+
+end
