isabelle/Chapter15_3_Typechecking.thy
@@ -1,0 +1,57 @@
+theory Chapter15_3_Typechecking
+imports Chapter15_2_Language
+begin
+
+inductive typecheck :: "type env \<Rightarrow> expr \<Rightarrow> type \<Rightarrow> bool" where 
+  tc_var [simp]: "lookup gam x = Some t \<Longrightarrow> typecheck gam (Var x) t"
+| tc_zero [simp]: "typecheck gam Zero Nat"
+| tc_suc [simp]: "typecheck gam e Nat \<Longrightarrow> typecheck gam (Suc e) Nat"
+| tc_iter [simp]: "typecheck gam et Nat \<Longrightarrow> typecheck gam e0 t \<Longrightarrow> typecheck (extend gam t) es t \<Longrightarrow>
+    typecheck gam (Iter et e0 es) t"
+| tc_lam [simp]: "is_type t1 \<Longrightarrow> typecheck (extend gam t1) e t2 \<Longrightarrow> 
+    typecheck gam (Lam t1 e) (Arrow t1 t2)"
+| tc_appl [simp]: "typecheck gam e1 (Arrow t2 t) \<Longrightarrow> typecheck gam e2 t2 \<Longrightarrow>
+    typecheck gam (Appl e1 e2) t"
+| tc_triv [simp]: "typecheck gam Triv Unit"
+| tc_pair [simp]: "typecheck gam e1 t1 \<Longrightarrow> typecheck gam e2 t2 \<Longrightarrow>
+    typecheck gam (Pair e1 e2) (Prod t1 t2)"
+| tc_projl [simp]: "typecheck gam e (Prod t1 t2) \<Longrightarrow> typecheck gam (ProjL e) t1"
+| tc_projr [simp]: "typecheck gam e (Prod t1 t2) \<Longrightarrow> typecheck gam (ProjR e) t2"
+| tc_abort [simp]: "is_type t \<Longrightarrow> typecheck gam e Void \<Longrightarrow> typecheck gam (Abort t e) t"
+| tc_case [simp]: "typecheck gam et (Sum t1 t2) \<Longrightarrow> typecheck (extend gam t1) el t \<Longrightarrow>
+    typecheck (extend gam t2) er t \<Longrightarrow> typecheck gam (Case et el er) t"
+| tc_inl [simp]: "is_type t1 \<Longrightarrow> is_type t2 \<Longrightarrow> typecheck gam e t1 \<Longrightarrow> 
+    typecheck gam (InL t1 t2 e) (Sum t1 t2)"
+| tc_inr [simp]: "is_type t1 \<Longrightarrow> is_type t2 \<Longrightarrow> typecheck gam e t2 \<Longrightarrow> 
+    typecheck gam (InR t1 t2 e) (Sum t1 t2)"
+| tc_strgen [simp]: "typecheck gam e t \<Longrightarrow> typecheck (extend gam t) e1 Nat \<Longrightarrow> 
+    typecheck (extend gam t) e2 t \<Longrightarrow> typecheck gam (Strgen t e e1 e2) Stream"
+| tc_hd [simp]: "typecheck gam e Stream \<Longrightarrow> typecheck gam (Hd e) Nat"
+| tc_tl [simp]: "typecheck gam e Stream \<Longrightarrow> typecheck gam (Tl e) Stream"
+
+inductive_cases [elim!]: "typecheck gam (Var x) t"
+inductive_cases [elim!]: "typecheck gam Zero t"
+inductive_cases [elim!]: "typecheck gam (Suc e) t"
+inductive_cases [elim!]: "typecheck gam (Iter et e0 es) t"
+inductive_cases [elim!]: "typecheck gam (Lam t1 e) t"
+inductive_cases [elim!]: "typecheck gam (Appl e1 e2) t"
+inductive_cases [elim!]: "typecheck gam Triv t"
+inductive_cases [elim!]: "typecheck gam (Pair e1 e2) t"
+inductive_cases [elim!]: "typecheck gam (ProjL e) t"
+inductive_cases [elim!]: "typecheck gam (ProjR e) t"
+inductive_cases [elim!]: "typecheck gam (Abort t1 e) t"
+inductive_cases [elim!]: "typecheck gam (Case et el er) t"
+inductive_cases [elim!]: "typecheck gam (InL t1 t2 e) t"
+inductive_cases [elim!]: "typecheck gam (InR t1 t2 e) t"
+inductive_cases [elim!]: "typecheck gam (Strgen t1 e e1 e2) t"
+inductive_cases [elim!]: "typecheck gam (Hd e) t"
+inductive_cases [elim!]: "typecheck gam (Tl e) t"
+
+lemma [simp]: "typecheck gam e t \<Longrightarrow> n in gam \<Longrightarrow> typecheck (extend_at n gam t') (insert n e) t"
+  by (induction gam e t arbitrary: n rule: typecheck.induct) fastforce+
+
+lemma [simp]: "typecheck (extend_at n gam t') e t \<Longrightarrow> n in gam \<Longrightarrow> typecheck gam e' t' \<Longrightarrow> 
+    typecheck gam (subst e' n e) t"
+  by (induction "extend_at n gam t'" e t arbitrary: n gam t' e' rule: typecheck.induct) fastforce+
+
+end
