isabelle/Chapter15_4_Evaluation.thy
@@ -1,0 +1,113 @@
+theory Chapter15_4_Evaluation
+imports Chapter15_3_Typechecking
+begin
+
+primrec is_val :: "expr \<Rightarrow> bool" where 
+  "is_val (Var v) = False"
+| "is_val Zero = True"
+| "is_val (Suc e) = is_val e"
+| "is_val (Iter et e0 es) = False"
+| "is_val (Lam t e) = True"
+| "is_val (Appl e1 e2) = False"
+| "is_val Triv = True"
+| "is_val (Pair e1 e2) = (is_val e1 \<and> is_val e2)"
+| "is_val (ProjL e) = False"
+| "is_val (ProjR e) = False"
+| "is_val (Abort t e) = False"
+| "is_val (Case et el er) = False"
+| "is_val (InL t1 t2 e) = is_val e"
+| "is_val (InR t1 t2 e) = is_val e"
+| "is_val (Strgen t e e1 e2) = True"
+| "is_val (Hd e) = False"
+| "is_val (Tl e) = False"
+
+inductive eval :: "expr \<Rightarrow> expr \<Rightarrow> bool" where 
+  eval_suc [simp]: "eval e e' \<Longrightarrow> eval (Suc e) (Suc e')"
+| eval_iter_1 [simp]: "eval et et' \<Longrightarrow> eval (Iter et e0 es) (Iter et' e0 es)"
+| eval_iter_2 [simp]: "eval (Iter Zero e0 es) e0"
+| eval_iter_3 [simp]: "is_val et \<Longrightarrow> eval (Iter (Suc et) e0 es) (subst (Iter et e0 es) first es)"
+| eval_appl_1 [simp]: "eval e1 e1' \<Longrightarrow> eval (Appl e1 e2) (Appl e1' e2)"
+| eval_appl_2 [simp]: "is_val e1 \<Longrightarrow> eval e2 e2' \<Longrightarrow> eval (Appl e1 e2) (Appl e1 e2')"
+| eval_appl_3 [simp]: "is_val e2 \<Longrightarrow> eval (Appl (Lam t2 e1) e2) (subst e2 first e1)"
+| eval_pair_1 [simp]: "eval e1 e1' \<Longrightarrow> eval (Pair e1 e2) (Pair e1' e2)"
+| eval_pair_2 [simp]: "is_val e1 \<Longrightarrow> eval e2 e2' \<Longrightarrow> eval (Pair e1 e2) (Pair e1 e2')"
+| eval_projl_1 [simp]: "eval e e' \<Longrightarrow> eval (ProjL e) (ProjL e')"
+| eval_projl_2 [simp]: "eval (ProjL (Pair e1 e2)) e1"
+| eval_projr_1 [simp]: "eval e e' \<Longrightarrow> eval (ProjR e) (ProjR e')"
+| eval_projr_2 [simp]: "eval (ProjR (Pair e1 e2)) e2"
+| eval_abort [simp]: "eval e e' \<Longrightarrow> eval (Abort t e) (Abort t e')"
+| eval_case_1 [simp]: "eval et et' \<Longrightarrow> eval (Case et el er) (Case et' el er)"
+| eval_case_2 [simp]: "is_val e \<Longrightarrow> eval (Case (InL t1 t2 e) el er) (subst e first el)"
+| eval_case_3 [simp]: "is_val e \<Longrightarrow> eval (Case (InR t1 t2 e) el er) (subst e first er)"
+| eval_inl [simp]: "eval e e' \<Longrightarrow> eval (InL t1 t2 e) (InL t1 t2 e')"
+| eval_inr [simp]: "eval e e' \<Longrightarrow> eval (InR t1 t2 e) (InR t1 t2 e')"
+| eval_hd1 [simp]: "eval e e' \<Longrightarrow> eval (Hd e) (Hd e')"
+| eval_hd2 [simp]: "eval (Hd (Strgen t e e1 e2)) (subst e first e1)"
+| eval_tl1 [simp]: "eval e e' \<Longrightarrow> eval (Tl e) (Tl e')"
+| eval_tl2 [simp]: "eval (Tl (Strgen t e e1 e2)) (Strgen t (subst e first e2) e1 e2)"
+
+lemma canonical_nat: "is_val e \<Longrightarrow> typecheck gam e Nat \<Longrightarrow> e = Zero \<or> (\<exists>e'. e = Suc e')"
+  by (induction e) auto
+
+lemma canonical_arrow: "is_val e \<Longrightarrow> typecheck gam e (Arrow t1 t2) \<Longrightarrow> \<exists>e'. e = Lam t1 e'"
+  by (induction e) auto
+
+lemma canonical_unit: "is_val e \<Longrightarrow> typecheck gam e Unit \<Longrightarrow> e = Triv"
+  by (induction e) auto
+
+lemma canonical_prod: "is_val e \<Longrightarrow> typecheck gam e (Prod t1 t2) \<Longrightarrow> \<exists>e1 e2. e = Pair e1 e2"
+  by (induction e) auto
+
+lemma canonical_void: "is_val e \<Longrightarrow> typecheck gam e Void \<Longrightarrow> False"
+  by (induction e) auto
+
+lemma canonical_sum: "is_val e \<Longrightarrow> typecheck gam e (Sum t1 t2) \<Longrightarrow> 
+    (\<exists>e'. e = InL t1 t2 e') \<or> (\<exists>e'. e = InR t1 t2 e')"
+  by (induction e) auto
+
+lemma canonical_stream: "is_val e \<Longrightarrow> typecheck gam e Stream \<Longrightarrow> \<exists>t e' e1 e2. e = Strgen t e' e1 e2"
+  by (induction e) auto
+
+theorem preservation: "eval e e' \<Longrightarrow> typecheck gam e t \<Longrightarrow> typecheck gam e' t"
+  by (induction e e' arbitrary: t rule: eval.induct) fastforce+
+
+theorem progress: "typecheck gam e t \<Longrightarrow> gam = empty_env \<Longrightarrow> is_val e \<or> (EX e'. eval e e')"
+  proof (induction gam e t rule: typecheck.induct)
+  case tc_var
+    thus ?case by simp
+  next case tc_zero
+    thus ?case by simp
+  next case tc_suc
+    thus ?case by (metis eval_suc is_val.simps(3))
+  next case tc_iter
+    thus ?case by (metis eval_iter_1 eval_iter_2 eval_iter_3 is_val.simps(3) canonical_nat)
+  next case tc_lam
+    thus ?case by simp
+  next case tc_appl
+    thus ?case by (metis eval_appl_1 eval_appl_2 eval_appl_3 canonical_arrow)
+  next case tc_triv
+    thus ?case by simp
+  next case tc_pair
+    thus ?case by (metis eval_pair_1 eval_pair_2 is_val.simps(8))
+  next case tc_projl
+    thus ?case by (metis eval_projl_1 eval_projl_2 canonical_prod)
+  next case tc_projr
+    thus ?case by (metis eval_projr_1 eval_projr_2 canonical_prod)
+  next case tc_abort
+    thus ?case by (metis eval_abort canonical_void)
+  next case tc_case
+    thus ?case 
+      by (metis eval_case_1 eval_case_2 eval_case_3 is_val.simps(13) is_val.simps(14) canonical_sum)
+  next case tc_inl
+    thus ?case by (metis eval_inl is_val.simps(13))
+  next case tc_inr
+    thus ?case by (metis eval_inr is_val.simps(14))
+  next case tc_strgen
+    thus ?case by simp
+  next case tc_hd
+    thus ?case by (metis eval_hd1 eval_hd2 canonical_stream)
+  next case tc_tl
+    thus ?case by (metis eval_tl1 eval_tl2 canonical_stream)
+  qed
+
+end
