isabelle/CompileAll.thy
@@ -4,14 +4,19 @@ imports
   Chapter08_3_Evaluation
   Chapter09_3_Evaluation
   Chapter10_3_Evaluation
-  Chapter11_3_Evaluation
-  Chapter12_4_Evaluation
+  Chapter11_4_Abbreviations
+  Chapter14_4_Abbreviations
+
+(*
+
   Chapter15_3_Evaluation
   Chapter16_5_Abbreviation
   Chapter17
   Chapter18_3_Evaluation
   Chapter20_3_Evaluation
   Chapter21_3_Evaluation
+
+*)
 begin
 
 datatype OK = OK
