isabelle/Name.thy
@@ -1,0 +1,9 @@
+theory Name
+imports Main
+begin
+
+typedecl name
+
+type_synonym 'a env = "name \<rightharpoonup> 'a"
+
+end
